Fomega/Ctx.lean
@@ -5,18 +5,19 @@ namespace Fomega
 
   abbrev Ctx := List Term
 
-  namespace Ctx
+  @[simp]
+  def nth : List Term -> Nat -> Term
+  | [], _ => .none
+  | .cons h _, 0 => h
+  | .cons _ t, n + 1 => nth t n
 
-    def apply : Subst Term -> Ctx -> Ctx
-    | _, [] => []
-    | σ, .cons h t => .cons ([σ]h) (apply ^σ t)
-
-    def beta : Ctx -> Term -> Ctx
-    | s, t => apply ((.replace t) :: (r#I)) s
-
-  end Ctx
+  @[simp]
+  def dnth : List Term -> Nat -> Term
+  | [], _ => .none
+  | .cons h _, 0 => [S]h
+  | .cons _ t, n + 1 => [S](dnth t n)
 
 end Fomega
 
-notation:90 "[" σ "]" t:89 => Fomega.Ctx.apply σ t
-notation:90 s:90 "β[" t "]" => Fomega.Ctx.beta s t
+infix:1000 "@" => Fomega.nth
+infix:1000 "d@" => Fomega.dnth
