Fomega/FreeVars.lean
@@ -1,0 +1,103 @@
+import Common
+import Fomega.Proof
+
+namespace Fomega
+
+  inductive IsFreeVar : Nat -> ∀ Γ t A, Proof Γ t A -> Prop where
+  | var1 :
+    (p1 : A = Γ d@ x) ->
+    IsFreeVar n Γ A (.const K) p2 ->
+    IsFreeVar n Γ (.bound K x) A (.var p1 p2)
+  | var2 :
+    (p1 : A = Γ d@ n) ->
+    (p2 : Γ ⊢ A : Term.const K) ->
+    IsFreeVar n Γ (.bound K n) A (.var p1 p2)
+  | pi1 :
+    IsFreeVar n Γ A (.const K) p1 ->
+    (p2 : (A::Γ) ⊢ B : ★) ->
+    IsFreeVar n Γ (.all mf A B) ★ (.pi p1 p2)
+  | pi2 :
+    (p1 : Γ ⊢ A : Term.const K) ->
+    IsFreeVar (n + 1) (A::Γ) B ★ p2 ->
+    IsFreeVar n Γ (.all mf A B) ★ (.pi p1 p2)
+  | tpi1 :
+    IsFreeVar n Γ A □ p1 ->
+    (p2 : (A::Γ) ⊢ B : □) ->
+    IsFreeVar n Γ (.all mf A B) □ (.tpi p1 p2)
+  | tpi2 :
+    (p1 : Γ ⊢ A : □) ->
+    IsFreeVar (n + 1) (A::Γ) B □ p2 ->
+    IsFreeVar n Γ (.all mf A B) □ (.tpi p1 p2)
+  | lam1 :
+    IsFreeVar n Γ (.all mf A B) (.const K) p1 ->
+    (p2 : (A::Γ) ⊢ t : B) ->
+    IsFreeVar n Γ (.lam mf A t) (.all mf A B) (.lam p1 p2)
+  | lam2 :
+    (p1 : Γ ⊢ Term.all mf A B : Term.const K) ->
+    IsFreeVar (n + 1) (A::Γ) t B p2 ->
+    IsFreeVar n Γ (.lam mf A t) (.all mf A B) (.lam p1 p2)
+  | app1 :
+    IsFreeVar n Γ f (.all mf A B) p1 ->
+    (p2 : Γ ⊢ a : A) ->
+    (p3 : B' = (B β[a])) ->
+    IsFreeVar n Γ (.app mf f a) B' (.app p1 p2 p3)
+  | app2 :
+    (p1 : Γ ⊢ f : (.all mf A B)) ->
+    IsFreeVar n Γ a A p2 ->
+    (p3 : B' = (B β[a])) ->
+    IsFreeVar n Γ (.app mf f a) B' (.app p1 p2 p3)
+  | conv1 :
+    IsFreeVar n Γ t A p1 ->
+    (p2 : Γ ⊢ B : Term.const K) ->
+    (p3 : A === B) ->
+    IsFreeVar n Γ t B (.conv p1 p2 p3)
+  | conv2 :
+    (p1 : Γ ⊢ t : A) ->
+    IsFreeVar n Γ B (.const K) p2 ->
+    (p3 : A === B) ->
+    IsFreeVar n Γ t B (.conv p1 p2 p3)
+
+
+  -- n ∈ ([^{n}S]t)
+  theorem fv_missing : (p : Γ ⊢ ([^{n}S]t) : ([^{n}S]T)) -> ¬ (IsFreeVar n Γ ([^{n}S]t) ([^{n}S]T) p) := by
+  intro j h
+  generalize sdef : [^{n}S]t = s at j
+  generalize Adef : [^{n}S]T = A at j
+  induction h generalizing t T
+  case var1 => sorry
+  case var2 => sorry
+  case pi1 n Γ' A' K p1 B h p2 ih =>
+    cases t <;> simp at sdef
+    case _ K' x =>
+      have lem := @Term.rep_n_S_exists n x
+      cases lem; case _ z h => rw [h] at sdef; simp at sdef
+    case _ m r1 r2 => apply @ih r1 (.const K) sdef.2.1 (by simp)
+  case pi2 => sorry
+  case tpi1 => sorry
+  case tpi2 => sorry
+  case lam1 => sorry
+  case lam2 => sorry
+  case app1 n Γ' f A' B p1 a B' h p2 p3 ih =>
+    cases t <;> simp at sdef
+    case _ K' x =>
+      have lem := @Term.rep_n_S_exists n x
+      cases lem; case _ z h => rw [h] at sdef; simp at sdef
+    case _ m r1 r2 =>
+      cases p1
+      case _ x K' j1 j2 =>
+        sorry
+      case _ K' t j1 j2 =>
+        have rdef := sdef.2.1
+        cases r1 <;> simp at rdef
+        case _ => sorry
+        case _ => sorry
+      case _ => sorry
+      case _ => sorry
+  case app2 => sorry
+  case conv1 => sorry
+  case conv2 => sorry
+
+
+
+
+end Fomega
