Fomega/PreProof.lean
@@ -1,0 +1,121 @@
+
+import Common
+import Fomega.Proof
+
+namespace Fomega
+
+  inductive IsPreProof : Term -> Prop where
+  | ax : IsPreProof ★
+  | bound : IsPreProof (.bound K x)
+  | all : IsPreProof A -> IsPreProof B -> IsPreProof (.all mf A B)
+  | lam : IsPreProof A -> IsPreProof t -> IsPreProof (.lam mf A t)
+  | app : IsPreProof f -> IsPreProof a -> IsPreProof (.app mf f a)
+
+  namespace IsPreProof
+    theorem from_subst : IsPreProof ([σ]t) -> IsPreProof t := by
+    intro j
+    induction t generalizing σ <;> (try (simp at j; cases j))
+    case bound K x => constructor
+    case _ => constructor
+    case _ ih1 ih2 j1 j2 =>
+      constructor; apply ih1 j1; apply ih2 j2
+    case _ ih1 ih2 j1 j2 =>
+      constructor; apply ih1 j1; apply ih2 j2
+    case _ ih1 ih2 j1 j2 =>
+      constructor; apply ih1 j1; apply ih2 j2
+
+  theorem ren : IsPreProof t -> IsPreProof ([r#r]t) := by
+    intro j
+    induction j generalizing r <;> simp
+    case ax => constructor
+    case bound => constructor
+    case all _j1 _j2 ih1 ih2 =>
+      constructor; apply ih1
+      replace ih2 := @ih2 (Term.Ren.lift r)
+      simp at ih2; exact ih2
+    case lam _j1 _j2 ih1 ih2 =>
+      constructor; apply ih1
+      replace ih2 := @ih2 (Term.Ren.lift r)
+      simp at ih2; exact ih2
+    case app _j1 _j2 ih1 ih2 =>
+      constructor; apply ih1; apply ih2
+
+    theorem lift : (∀ n s, σ n = .replace s -> IsPreProof s) -> ∀ n s, ^σ n = .replace s -> IsPreProof s := by
+    intro h n s eq; simp at *
+    cases n <;> simp at eq
+    case _ n =>
+      unfold Term.Subst.compose at eq; simp at eq
+      generalize xdef : σ n = x at *
+      cases x <;> simp at *
+      case _ t =>
+        subst eq
+        replace h := h n t xdef
+        apply ren h
+
+    theorem subst : (∀ n s, σ n = .replace s -> IsPreProof s) -> IsPreProof t -> IsPreProof ([σ]t) := by
+    intro h j
+    induction j generalizing σ <;> simp
+    case ax => constructor
+    case bound K n =>
+      generalize xdef : σ n = x at *
+      cases x <;> simp
+      case _ => constructor
+      case _ t => apply h n t xdef
+    case all _j1 _j2 ih1 ih2 =>
+      constructor; apply ih1 h
+      replace ih2 := @ih2 (^σ) (lift h)
+      simp at ih2; exact ih2
+    case lam _j1 _j2 ih1 ih2 =>
+      constructor; apply ih1 h
+      replace ih2 := @ih2 (^σ) (lift h)
+      simp at ih2; exact ih2
+    case app _j1 _j2 ih1 ih2 =>
+      constructor; apply ih1 h; apply ih2 h
+
+    theorem beta : IsPreProof b -> IsPreProof t -> IsPreProof (b β[t]) := by
+    simp; intro j1 j2
+    apply subst
+    case _ =>
+      intro n s eq
+      cases n <;> simp at *
+      subst eq; exact j2
+    case _ => exact j1
+
+    theorem from_proof : Γ ⊢ t : A -> IsPreProof t := by
+    intro j; induction j
+    case ax => constructor
+    case var => constructor
+    case pi _j1 _j2 ih1 ih2 => constructor <;> simp [*]
+    case tpi => constructor <;> simp [*]
+    case lam j1 _j2 ih1 ih2 => constructor; cases ih1; all_goals simp [*]
+    case app => constructor <;> simp [*]
+    case conv => simp [*]
+
+    theorem conv : IsPreProof A -> A === B -> IsPreProof B := by
+    intro j h
+    induction h
+    case ax => constructor
+    case bound => constructor
+    case all_congr _j1 _j2 ih1 ih2 =>
+      cases j; constructor <;> simp [*]
+    case lam_congr _j1 _j2 ih1 ih2 =>
+      cases j; constructor <;> simp [*]
+    case lam_eta _j ih =>
+      replace ih := ih j
+      cases ih
+      case _ j1 j2 =>
+        cases j2
+        case _ j2 j3 =>
+          apply IsPreProof.from_subst j2
+    case app_congr _j1 _j2 ih1 ih2 =>
+      cases j; constructor <;> simp [*]
+    case app_beta _j ih =>
+      cases j
+      case _ j1 j2 =>
+        cases j1
+        case _ j1 j3 =>
+          apply ih (IsPreProof.beta j3 j2)
+
+  end IsPreProof
+
+end Fomega
